trying to prove hoare_seq_soundness, adding auxilliart updates

code/Soundness.v
@@ -2,6 +2,8 @@ Require Import AB.Imp8.
 Require Import AB.Denotation.
 Require Import AB.HoareLogic.
 
+Open Scope list_scope.
+
 Import Assertion_D.
 Export Abstract_Pretty_Printing.
 
@@ -11,7 +13,7 @@ Import Hoare_Logic.
 Definition valid (Tr: hoare_triple): Prop :=
   match Tr with
   | Build_hoare_triple P c Q T =>
-      exists a1 a2 N,
+      exists a1 a2 N, 0 < a1 /\ 0 < a2 /\ 0 < N /\
       forall La st1 st2 t,
         (st1, La) |== P ->
         ceval c st1 t st2 ->
@@ -20,12 +22,18 @@ Definition valid (Tr: hoare_triple): Prop :=
 
 Notation "|==  Tr" := (valid Tr) (at level 91, no associativity).
 
-(* The p should be 1 *)
-Lemma hoare_skip_sound : forall P p n,
-  |== {{P}} Skip {{P}} $ BigTheta p n.
+(** Soundness Proof *)
+
+Lemma hoare_skip_sound : forall P n,
+  |== {{P}} Skip {{P}} $ BigTheta nil n.
 Proof.
   unfold valid.
-  exists 1, 1, 0.
+  exists 1, 1, 1.
+  
+  split. omega.
+  split. omega.
+  split. omega.
+  
   intros.
   simpl in H0.
   unfold skip_sem in H0.
@@ -39,12 +47,92 @@ Proof.
     unfold ab_eval.
     intros.
     remember (La n) as n'.
-    admit. (* after poly is fully defined *)
+    simpl. omega.
   }
-Admitted.
+Qed.
+
+Lemma Assertion_sub_spec: forall st1 st2 La (P: Assertion) (X: var) (E: aexp'),
+  st2 X = aexp'_denote (st1, La) E ->
+  (forall Y : var, X <> Y -> st1 Y = st2 Y) ->
+  ((st1, La) |== P[ X |-> E]) <-> ((st2, La) |== P).
+(* FILL IN HERE *) Admitted.
+
+Lemma hoare_asgn_bwd_sound : forall P (X: var) (E: aexp) n,
+  |== {{ P [ X |-> E] }} X ::= E {{ P }} $ BigTheta (1::nil) n.
+Proof.
+  unfold valid.
+  exists 1, 1, 1.
+  
+  split. omega.
+  split. omega.
+  split. omega.
+  
+  intros.
+  simpl in *.
+  destruct H0, H1.
+  split.
+  {
+    pose proof aeval_aexp'_denote st1 La E.
+    rewrite H3 in H0.
+    pose proof Assertion_sub_spec st1 st2 _ P _ _ H0 H1.
+    tauto.
+  }
+  {
+    intros.
+    omega.
+  }
+Qed.
 
 Lemma hoare_seq_sound_bigtheta : forall (P Q R: Assertion) (c1 c2: com) (p1 p2 : poly) (n : logical_var),
   |== {{P}} c1 {{Q}} $ BigTheta p1 n ->
   |== {{Q}} c2 {{R}} $ BigTheta p2 n ->
   |== {{P}} c1;;c2 {{R}} $ BigTheta (poly_add p1 p2) n.
-Admitted.
+Proof.
+  unfold valid.
+  intros.
+  destruct H as [a1 [a2 [N [h1 [h2 [h3 ?]]]]]].
+  destruct H0 as [a1' [a2' [N' [h1' [h2' [h3' ?]]]]]].
+  simpl in *.
+  exists (Z.min a1 a1'), (Z.max a2 a2'), (Z.max N N').
+  
+  split. apply (Z.min_glb_lt _ _ _ h1 h1').
+  split. pose proof Z.le_max_l a2 a2'. omega.
+  split. pose proof Z.le_max_l N N'. omega.
+  
+  intros.
+  unfold seq_sem in H2.
+  destruct H2 as [t1 [t2 [st3 [? [? ?]]]]].
+  specialize (H _ _ _ _ H1 H2) as [? ?].
+  specialize (H0 _ _ _ _ H H3) as [? ?].
+  split.
+  {
+    exact H0.
+  }
+  {
+    intros.
+    pose proof Z.max_lub_l _ _ _ H7;
+    pose proof Z.max_lub_r _ _ _ H7;
+    clear H7.
+    specialize (H5 H8); clear H8.
+    specialize (H6 H9); clear H9.
+    clear H1 H2 H3 H H0.
+    destruct H5, H6.
+    split.
+    - rewrite poly_add_eval_comm.
+      
+  }
+
+
+
+
+
+
+
+
+
+
+
+
+
+
+(** [] *)
